Reworking

theories/Group.v
@@ -2,88 +2,123 @@ From Nominal Require Export Prelude.
 
 (** *Group operations *)
 Class Neutral A := neutral : A.
-Hint Mode Neutral ! : typeclass_instances.
-Notation ε := neutral.
+#[global] Hint Mode Neutral ! : typeclass_instances.
+Notation ɛ := neutral.
+Notation "ɛ@{ A }" := (@neutral A _) (only parsing) : nominal_scope.
 
 Class Operator A := op: A → A → A.
-Hint Mode Operator ! : typeclass_instances.
-(* Instance: Params (@op) 2 := {}. *)
+#[global] Hint Mode Operator ! : typeclass_instances.
+Instance: Params (@op) 2 := {}.
+
 Infix "+" := op : nominal_scope.
 Notation "(+)" := op (only parsing) : nominal_scope.
+(* Notation "( +@{ A } )" := (@op A _) (only parsing) : nominal_scope. *)
 Notation "(+ x )" := (op x) (only parsing) : nominal_scope.
 Notation "( x +)" := (λ y, op y x) (only parsing) : nominal_scope.
 
 Class Inverse A := inv : A → A.
-Hint Mode Inverse ! : typeclass_instances.
-(* Instance: Params (@inv) 1 := {}. *)
+#[global] Hint Mode Inverse ! : typeclass_instances.
+Instance: Params (@inv) 1 := {}.
+
 Notation "- x" := (inv x) : nominal_scope.
 Notation "(-)" := inv (only parsing) : nominal_scope.
-Notation "x - y" := (x + (-y))%nom (only parsing) : nominal_scope.
+(* Notation "( -@{ A } )" := (@inv A _) (only parsing) : nominal_scope. *)
+Notation "x - y" := (x + (-y))%nom : nominal_scope.
 
-Section Group.
-  Context A `{Equiv A, !Equivalence(≡@{A}), Neutral A, Operator A, Inverse A}.
+Section GroupDef.
+  Context (A : Type) `{Ntr: Neutral A, Opr: Operator A, Inv: Inverse A, EqG: Equiv A}.
 
   Class Group: Prop := {
-    group_assoc : ∀ x y z, x + (y + z) ≡@{A} (x + y) + z;
-    group_left_id : ∀ x, ε + x ≡@{A} x;
-    group_right_id : ∀ x, x + ε ≡@{A} x;
-    group_left_inv : ∀ x, (-x) + x ≡@{A} ε;
-    group_right_inv : ∀ x, x - x ≡@{A} ε;
-
     group_setoid :> Equivalence(≡@{A});
     group_op_proper :> Proper ((≡@{A}) ==> (≡@{A}) ==> (≡@{A})) (+);
-    group_inv_proper :> Proper ((≡@{A}) ==> (≡@{A})) (-)
+    group_inv_proper :> Proper ((≡@{A}) ==> (≡@{A})) (-);
+
+    group_assoc : ∀ x y z, x + (y + z) ≡@{A} (x + y) + z;
+
+    group_left_id : ∀ x, ɛ + x ≡@{A} x;
+    group_right_id : ∀ x, x + ɛ ≡@{A} x;
+
+    group_left_inv : ∀ x, (-x) + x ≡@{A} ɛ;
+    group_right_inv : ∀ x, x - x ≡@{A} ɛ;
   }.
-End Group.
+End GroupDef.
+(* #[global] Hint Mode Group ! - - - -: typeclass_instances. *)
 
-Arguments group_assoc {A AEq NA OA IA GA}: rename.
-Arguments group_left_id {A AEq NA OA IA GA}: rename.
-Arguments group_right_id {A AEq NA OA IA GA}: rename.
-Arguments group_left_inv {A AEq NA OA IA GA}: rename.
-Arguments group_right_inv {A AEq NA OA IA GA}: rename.
-Arguments group_op_proper {A AEq NA OA IA GA}: rename.
-Arguments group_inv_proper {A AEq NA OA IA GA}: rename.
+Arguments group_assoc {_ _ _ _ _ Grp} : rename.
+Arguments group_left_id {_ _ _ _ _ Grp} : rename.
+Arguments group_right_id {_ _ _ _ _ Grp} : rename.
+Arguments group_left_inv {_ _ _ _ _ Grp} : rename.
+Arguments group_right_inv {_ _ _ _ _ Grp} : rename.
+Arguments group_op_proper {_ _ _ _ _ Grp} : rename.
+Arguments group_inv_proper {_ _ _ _ _ Grp} : rename.
 
+(* Basic group theory properties *)
 Section GroupProperties.
   Context `{Group G}.
 
-  Corollary group_inv_involutive (x: G): x ≡ --x.
+  Corollary group_inv_involutive (x: G): --x ≡ x.
   Proof with auto.
-    rewrite <-group_left_id at 1; rewrite <-group_left_inv, <-group_assoc, group_left_inv, group_right_id;
-      reflexivity.
+    rewrite <-(group_left_id x) at 2;
+     rewrite <-group_left_inv, <-group_assoc, group_left_inv, group_right_id...
   Qed.
 
-  Corollary inv_neutral: ε ≡@{G} -ε.
+  Corollary inv_neutral: -ɛ ≡@{G} ɛ.
   Proof with auto.
-    rewrite <-group_left_inv at 2; rewrite group_right_id, <-group_inv_involutive...
+    rewrite <-group_left_inv at 1; rewrite group_right_id, group_inv_involutive...
   Qed.
 
-  (* Corollary group_inv_inj (x y: G): x ≡ y → (-x) ≡ (-y). *)
-  (* Proof. apply group_inv_proper. Qed. *)
+  Corollary group_inv_inj (x y: G): x ≡ y → (-x) ≡ (-y).
+  Proof. apply group_inv_proper. Qed.
 End GroupProperties.
 
-(** *Group action *)
-Class Action `(Group A) X := action: A → X → X.
-(* Instance: Params (@action) 2 := {}. *)
-Infix "∙" := action (at level 60, right associativity) : nominal_scope.
-Notation "(∙)" := action (only parsing) : nominal_scope.
-Notation "(∙ x )" := (action x) (only parsing) : nominal_scope.
-Notation "( x ∙)" := (λ y, action y x) (only parsing): nominal_scope.
+(* Group Action  *)
+Class Action (* `{Grp: Group A} *) A X := action: A -> X -> X.
+#[global] Hint Mode Action ! ! : typeclass_instances.
+(*
+CAUSA PROBLEMAS COM REESCRITA ENVOLVENDO action (- p)
+Instance: Params (@action) 2 := {}. 
+*)
+
+Infix "•" := action (at level 60, right associativity) : nominal_scope.
+Notation "(•)" := action (only parsing) : nominal_scope.
+(* Notation "( •@{ A X } )" := (@action A X _) (only parsing) : nominal_scope. *)
+Notation "(• x )" := (action x) (only parsing) : nominal_scope.
+Notation "( x •)" := (λ y, action y x) (only parsing): nominal_scope.
 
 Section GroupAction.
-  Context A X `{Action A X, Equiv X, !Equivalence(≡@{X})}.
+  Context (A X: Type) `{Grp: Group A, Act : Action A X, Equiv X}.
 
-  Class GroupAction: Prop := {
-    action_id : ∀ (x: X), ε ∙ x ≡@{X} x;
-    action_compat: ∀ (p q: A) (r: X), p ∙ (q ∙ r) ≡@{X} (q + p) ∙ r;
+  Class GAction: Prop := {
+    gact_group :> Group A;
+    gact_setoid :> Equivalence(≡@{X});
+    gact_proper :> Proper ((≡@{A}) ==> (≡@{X}) ==> (≡@{X})) (•);
 
-    (* action_group :> Group A; *)
-    action_setoid :> Equivalence(≡@{X});
-    action_proper :> Proper ((≡@{A}) ==> (≡@{X}) ==> (≡@{X})) (∙)
+    gact_id : ∀ (x: X), ɛ@{A} • x ≡@{X} x;
+    gact_compat: ∀ (p q: A) (x: X), p • (q • x) ≡@{X} (q + p) • x
   }.
 End GroupAction.
 
-Arguments GroupAction (A X) {AEq AN AO AI AG ActAX XEq}: rename.
-Arguments action_compat {A X AEq NA OA IA GA ActAX XEq GActAX}: rename.
-Arguments action_id {A X AEq NA OA IA GA ActAX XEq GActAX}: rename.
-Arguments action_proper {A X AEq NA OA IA GA ActAX XEq GActAX}: rename.
+Arguments gact_compat {_ _ _ _ _ _ _ EqX GAct} : rename.
+Arguments gact_id {_ _ _ _ _ _ _ EqX GAct} : rename.
+Arguments gact_proper {_ _ _ _ _ _ _ EqX GAct} : rename.
+
+Section GroupActionProperties.
+  Context `{GAction G X}.
+
+  Corollary perm_left_inv (x: X) (p : G): (-p) • p • x ≡ x.
+  Proof. rewrite gact_compat, group_right_inv, gact_id; auto. Qed.
+
+  Corollary perm_rigth_inv (x: X) (p : G): p • (-p) • x ≡ x.
+  Proof. rewrite gact_compat, group_left_inv, gact_id; auto. Qed.
+
+  Lemma perm_iff (x y: X) (p : G): p • x ≡ y <-> x ≡ (-p) • y.
+  Proof.
+    split; intros A;
+      [rewrite <-A, perm_left_inv | rewrite A, perm_rigth_inv]; auto.
+  Qed.
+
+  Lemma perm_inj (x y: X) (p : G): p • x ≡ p • y <-> x ≡ y.
+  Proof.
+    split; intros A; [apply perm_iff in A; rewrite <-(perm_left_inv y p) | rewrite A]; auto.
+  Qed.
+End GroupActionProperties.
