theories/Nominal.v
@@ -1,7 +1,7 @@
 From Nominal Require Export Perm.
 
-Class Support A := support: A -> nset.
-Hint Mode Support ! : typeclass_instances.
+Class Support A := support: A -> nameset.
+#[global] Hint Mode Support ! : typeclass_instances.
 
 Section Nominal.
   Context X `{PX: Perm X, S: Support X}.
@@ -9,35 +9,37 @@ Section Nominal.
   Class Nominal: Prop := {
     nom_perm :> Perm X;
     support_spec : forall (x: X) (a b: name),
-        a ∉ (support x) -> b ∉ (support x) -> [(a,b)] ∙ x ≡@{X} x
+        a ∉ (support x) -> b ∉ (support x) -> [(a,b)] • x ≡@{X} x
 }.
 End Nominal.
 
+#[global] Hint Mode Nominal ! - - - : typeclass_instances.
 Arguments support_spec {X XPAct XEq XS XN}: rename.
 
 (* Freshness *)
-Definition fresh_e `{Nominal X} (a: name) (x: X) :=
-  exists b, b ∉ support x /\ [(a,b)] ∙ x ≡ x.
+Definition fresh_e `{Nominal X} (a: Name) (x: X) :=
+  exists b, b ∉ support x /\ [(a,b)] • x ≡ x.
 
-Definition fresh_a `{Nominal X} (a: name) (x: X) :=
-  forall b, b ∉ support x -> [(a,b)] ∙ x ≡ x.
+Definition fresh_a `{Nominal X} (a: Name) (x: X) :=
+  forall b, b ∉ support x -> [(a,b)] • x ≡ x.
 
 (* Infix "#" := freshness (at level 50). *)
 Infix "#ₑ" := fresh_e (at level 50).
 Infix "#ₐ" := fresh_a (at level 50).
 
-Lemma some_any `{Nominal X} (a: name) (x: X) : a #ₑ x <-> a #ₐ x.
+Lemma some_any `{Nominal X} (a: Name) (x: X) : a #ₑ x <-> a #ₐ x.
 Proof.
   split.
   - intros [b [SB HH]] c SC; destruct (decide (c = a)), (decide (c = b)); subst; auto.
-    + rewrite swap_equiv_neutral; apply action_id.
-    + rewrite swap_expand with (b := b); try rewrite <-2!action_compat, HH, (support_spec _ b c); auto.
+    + rewrite swap_equiv_neutral; apply gact_id.
+    + rewrite swap_expand with (b := b); try rewrite <-2!gact_compat, HH, (support_spec _ b c); auto.
   - intros HH; exists (fresh (support x)); split.
     + apply is_fresh.
     + apply HH, is_fresh.
 Qed.
 
-Lemma support_fresh_e `{Nominal X} a (x: X): a ∉ support x -> a #ₑ x.
+Lemma support_fresh_e `{Nominal X} a (x: X):
+  a ∉ support x -> a #ₑ x.
 Proof.
   intros; exists a; split; [idtac | rewrite swap_equiv_neutral; apply action_id]; auto.
 Qed.
