theories/Atom.v
@@ -1,0 +1,54 @@
+From Nominal Require Export Prelude.
+From stdpp Require Import listset countable infinite.
+
+Module Type ATOMIC.
+  Parameter t : Set.
+
+  Axiom dec : EqDecision t.
+  Axiom inf : Infinite t.
+End ATOMIC.
+
+Module Atom : ATOMIC.
+  Definition t := nat.
+
+  Instance dec : EqDecision t := nat_eq_dec.
+  Instance inf : Infinite t := nat_infinite.
+End Atom.
+#[global] Existing Instances Atom.dec Atom.inf.
+
+From elpi Require Import elpi.
+
+(* Class Atomic A := { dec :> EqDecision A; inf :> Infinite A }.
+Global Hint Mode Atomic ! : typeclass_instances.
+Arguments dec {_ _} _ _ : simpl never, assert.
+Arguments inf {_ _} : simpl never, assert.
+
+Definition Name : Set := nat.
+Instance name_atomic : Atomic Name. Proof. split; typeclasses eauto. Qed.
+
+Arguments Name : simpl never, assert.
+#[global] Opaque Name.
+*)
+
+Elpi Db atom.sort.db lp:{{
+  pred atom-sort o:id.
+
+  :name "atom.fail"
+  atom-sort _ :- coq.error "NOMINAL-ERROR: No atom-sort defined.".
+}}.
+
+(* Define new atomic name *)
+Elpi Command declare_name.
+Elpi Accumulate Db atom.sort.db.
+Elpi Accumulate declare_name lp:{{
+  main [str X] :-
+    coq.elpi.accumulate _ "atom.sort.db" (clause _ (before "atom.fail") (atom-sort X)),
+    @global! => coq.notation.add-abbreviation X 0 {{ Atom.t }} ff _.
+
+  main _ :- coq.say "Usage: declare_name [name]".
+}}.
+Elpi Typecheck.
+
+Elpi declare_name name.
+
+Notation nameset := (listset name).
